CBPV/Soundness.lean
@@ -11,17 +11,17 @@ open Nat ValType ComType Val Com
 @[simp]
 def semK (Γ : Ctxt) {δ} (Δ : Dtxt δ) k₁ k₂ B₁ B₂ :=
   ∀ {σ τ}, Γ ⊨ σ ~ τ →
-  ∀ {js₁ js₂}, Δ ⊨ js₁ ~ js₂ →
+  ∀ {φ ψ}, Δ ⊨ φ ~ ψ →
   ∀ {n₁ n₂}, (n₁, n₂) ∈ ⟦B₁⟧ᵉ →
-  (rejoin ((substK σ k₁) [n₁]) js₁, rejoin ((substK τ k₂) [n₂]) js₂) ∈ ⟦B₂⟧ᵉ
+  (rejoin ((substK σ k₁) [n₁]) φ, rejoin ((substK τ k₂) [n₂]) ψ) ∈ ⟦B₂⟧ᵉ
 notation:40 Γ:41 "∣" Δ:41 "⊨" k₁:41 "~" k₂:41 "∶" B₁:41 "⇒" B₂:41 => semK Γ Δ k₁ k₂ B₁ B₂
 
 namespace semK
 
 theorem weaken {Γ δ} {Δ : Dtxt δ} {k₁ k₂ A B₁ B₂} (h : Γ ∣ Δ ⊨ k₁ ~ k₂ ∶ B₁ ⇒ B₂) : Γ ∷ A ∣ Δ ⊨ renameK succ k₁ ~ renameK succ k₂ ∶ B₁ ⇒ B₂ := by
-  intro σ τ hστ js₁ js₂ hjs n₁ n₂ hn
+  intro σ τ hστ φ ψ hφψ n₁ n₂ hn
   rw [substRenameK, substRenameK]
-  exact h (semCtxt.rename wRenameSucc hστ) hjs hn
+  exact h (semCtxt.rename wRenameSucc hστ) hφψ hn
 
 /-*--------------------------------------------------------------
   Fundamental theorem for semantic equivalence of continuations
@@ -31,33 +31,33 @@ def nil {Γ δ B} {Δ : Dtxt δ} : Γ ∣ Δ ⊨ .nil ~ .nil ∶ B ⇒ B :=
   λ _ _ _ _ ↦ ℰ.bwdsRejoin .refl .refl
 
 def fst {Γ δ} {Δ : Dtxt δ} {k₁ k₂ B₁ B₂ B₃} (h : Γ ∣ Δ ⊨ k₁ ~ k₂ ∶ B₁ ⇒ B₃) : Γ ∣ Δ ⊨ .fst k₁ ~ .fst k₂ ∶ Prod B₁ B₂ ⇒ B₃ := by
-  intro σ τ hστ js₁ js₂ hjs n₁ n₂ hn; simp
+  intro σ τ hστ φ ψ hφψ n₁ n₂ hn; simp
   have ⟨n₁₁, n₁₂, n₂₁, n₂₂, rn₁, rn₂, hn₁⟩ := hn.fst
-  refine ℰ.bwds ?left ?right (h hστ hjs hn₁)
+  refine ℰ.bwds ?left ?right (h hστ hφψ hn₁)
   all_goals refine .rejoin (.plug ?_)
   case left  => rw [← @weakenJCom0 n₁₁]; exact .trans' (Evals.fst rn₁) (.once .π1)
   case right => rw [← @weakenJCom0 n₂₁]; exact .trans' (Evals.fst rn₂) (.once .π1)
 
 def snd {Γ δ} {Δ : Dtxt δ} {k₁ k₂ B₁ B₂ B₃} (h : Γ ∣ Δ ⊨ k₁ ~ k₂ ∶ B₂ ⇒ B₃) : Γ ∣ Δ ⊨ .snd k₁ ~ .snd k₂ ∶ Prod B₁ B₂ ⇒ B₃ := by
-  intro σ τ hστ js₁ js₂ hjs n₁ n₂ hn; simp
+  intro σ τ hστ φ ψ hφψ n₁ n₂ hn; simp
   have ⟨n₁₁, n₁₂, n₂₁, n₂₂, rn₁, rn₂, hn₂⟩ := hn.snd
-  refine ℰ.bwds ?left ?right (h hστ hjs hn₂)
+  refine ℰ.bwds ?left ?right (h hστ hφψ hn₂)
   all_goals refine .rejoin (.plug ?_)
   case left  => rw [← @weakenJCom0 n₁₂]; exact .trans' (Evals.snd rn₁) (.once .π2)
   case right => rw [← @weakenJCom0 n₂₂]; exact .trans' (Evals.snd rn₂) (.once .π2)
 
 theorem app {Γ δ} {Δ : Dtxt δ} {v w k₁ k₂ B₁ B₂} {A : ValType} (hA : Γ ⊨ v ~ w ∶ A) (h : Γ ∣ Δ ⊨ k₁ ~ k₂ ∶ B₁ ⇒ B₂) : Γ ∣ Δ ⊨ .app v k₁ ~ .app w k₂ ∶ Arr A B₁ ⇒ B₂ := by
-  intro σ τ hστ js₁ js₂ hjs n₁ n₂ hn; simp
+  intro σ τ hστ φ ψ hφψ n₁ n₂ hn; simp
   have ⟨_, _, rn₁, rn₂, hm⟩ := hn.lam_inv
-  refine ℰ.bwds ?left ?right (h hστ hjs (hm _ _ (hA hστ)))
+  refine ℰ.bwds ?left ?right (h hστ hφψ (hm _ _ (hA hστ)))
   all_goals refine .rejoin (.plug ?_)
   case left w _ => rw [← @weakenJCom0 (w⦃v⦃σ⦄⦄)]; exact .trans' (Evals.app rn₁) (.once .β)
   case right v  => rw [← @weakenJCom0 (v⦃w⦃τ⦄⦄)]; exact .trans' (Evals.app rn₂) (.once .β)
 
 theorem letin {Γ δ} {Δ : Dtxt δ} {m₁ m₂ A} {B : ComType} (h : Γ ∷ A ∣ Δ ⊨ m₁ ~ m₂ ∶ B) : Γ ∣ Δ ⊨ .letin m₁ ~ .letin m₂ ∶ F A ⇒ B := by
-  intro σ τ hστ js₁ js₂ hjs n₁ n₂ hn
+  intro σ τ hστ φ ψ hφψ n₁ n₂ hn
   have ⟨v, w, rn₁, rn₂, hA⟩ := hn.ret_inv
-  refine ℰ.bwds ?_ ?_ (h (semCtxt.cons hA hστ) hjs)
+  refine ℰ.bwds ?_ ?_ (h (semCtxt.cons hA hστ) hφψ)
   all_goals rw [← substUnion]; refine .rejoin ?_
   . exact .trans' (Evals.letin rn₁) (.once .ζ)
   . exact .trans' (Evals.letin rn₂) (.once .ζ)
@@ -77,8 +77,8 @@ theorem soundK {Γ δ} {Δ : Dtxt δ} {k B₁ B₂} (h : Γ ∣ Δ ⊢ k ∶ B�
 ----------------------------------------------*-/
 
 theorem semK.plug {Γ δ} {Δ : Dtxt δ} {n₁ n₂ k₁ k₂ B₁ B₂} (hk : Γ ∣ Δ ⊨ k₁ ~ k₂ ∶ B₁ ⇒ B₂) (hn : Γ ∣ ⬝ ⊨ n₁ ~ n₂ ∶ B₁) : Γ ∣ Δ ⊨ (k₁[n₁]) ~ (k₂[n₂]) ∶ B₂ := by
-  intro σ τ hστ js₁ js₂ hjs; rw [substPlug, substPlug]
-  exact hk hστ hjs (hn hστ .nil)
+  intro σ τ hστ φ ψ hφψ; rw [substPlug, substPlug]
+  exact hk hστ hφψ (hn hστ .nil)
 
 theorem semPlug {Γ δ} {Δ : Dtxt δ} {n₁ n₂ k B₁ B₂} (hk : Γ ∣ Δ ⊢ k ∶ B₁ ⇒ B₂) (hn : Γ ∣ ⬝ ⊨ n₁ ~ n₂ ∶ B₁) : Γ ∣ Δ ⊨ (k [ n₁ ]) ~ (k [ n₂ ]) ∶ B₂ :=
   semK.plug (soundK hk) hn
@@ -115,9 +115,9 @@ theorem semJumpPlug {Γ δ} {Δ : Dtxt δ} {k k' m n B₁ B₂} (hk : Γ ∣ Δ 
   case nil => cases e
   case letin hm =>
     simp at e; let ⟨ek, em⟩ := e; subst ek em
-    intro σ τ hστ js₁ js₂ hjs
+    intro σ τ hστ φ ψ hφψ
     let ⟨_, _, rn₁, rn₂, hA⟩ := (soundCom hn hστ .nil).ret_inv
-    refine ℰ.bwds ?left ?right (soundCom hm (semCtxt.cons hA hστ) hjs)
+    refine ℰ.bwds ?left ?right (soundCom hm (semCtxt.cons hA hστ) hφψ)
     all_goals refine .rejoin ?_; rw [← substUnion]
     case left => exact .trans' (Evals.letin rn₁) (.once .ζ)
     case right => exact .trans' (Evals.join (.trans' (Evals.letin rn₂) (.once .ζ))) (.once .γ)
@@ -126,7 +126,7 @@ theorem semJumpPlug {Γ δ} {Δ : Dtxt δ} {k k' m n B₁ B₂} (hk : Γ ∣ Δ 
     rename _ = _ => e
     refine ih ?_ e; constructor <;> assumption
 
-theorem semJumpA {Γ δ δ'} {Δ : Dtxt δ} {Δ' : Dtxt δ'} {k k' m m' B₁ B₂} (le : δ' ≤ δ) (mj : m.joinless) (hk : Γ ∣ Δ ⊢ k ∶ B₁ ⇒ B₂) (hm : Γ ∣ Δ' ⊢ m ∶ B₁) (e : k.jumpify = .yes k' m') :
+theorem semJumpCC {Γ δ δ'} {Δ : Dtxt δ} {Δ' : Dtxt δ'} {k k' m m' B₁ B₂} (le : δ' ≤ δ) (mj : m.joinless) (hk : Γ ∣ Δ ⊢ k ∶ B₁ ⇒ B₂) (hm : Γ ∣ Δ' ⊢ m ∶ B₁) (e : k.jumpify = .yes k' m') :
   Γ ∣ Δ ⊨ ⟦m⟧ₘ k # le ~ join m' (⟦m⟧ₘ k' # .step le) ∶ B₂ := by
   mutual_induction hm generalizing δ Δ k k' m' mj
   all_goals intro σ τ
@@ -152,7 +152,7 @@ theorem semJumpA {Γ δ δ'} {Δ : Dtxt δ} {Δ' : Dtxt δ'} {k k' m m' B₁ B�
     simp only [K.jumpify, e] at goal; exact goal ⟨⟩
   -- configuration cases
   case letin Γ _ n m A _ hn hm ihn ihm =>
-    intro hστ js₁ js₂ hjs; simp
+    intro hστ φ ψ hφψ; simp
     let ⟨nj, mj⟩ := mj
     have ⟨A', hk', hm'⟩ := wtK.jumpify hk e
     have ahm := ComWt.preservation le mj hk.weaken hm
@@ -161,18 +161,18 @@ theorem semJumpA {Γ δ δ'} {Δ : Dtxt δ} {Δ' : Dtxt δ'} {k k' m m' B₁ B�
     have aihm : Γ ∷ A ∣ Δ ⊨ (⟦ m ⟧ₘ renameK succ k # le) ~ join (renameCom (lift succ) m') (⟦ m ⟧ₘ renameK succ k' # .step le) ∶ B₂ :=
       λ {σ τ} ↦ ihm le mj hk.weaken (Jump.rename e) (σ := σ) (τ := τ)
     have hττ : Γ ⊨ τ ~ τ := semCtxt.trans hστ.sym hστ
-    have hjs₂₂ : Δ ⊨ js₂ ~ js₂ := semDtxt.trans hjs.sym hjs
-    apply ℰ.trans (ihn (zero_le δ) nj (wtK.letin ahm) rfl hστ hjs)
-    apply ℰ.trans (semCom.join aihm (soundCom ahn) hττ hjs₂₂)
-    apply ℰ.trans (joinJoin hm' ahm' ahn hττ hjs₂₂); simp
+    have hψ₂ : Δ ⊨ ψ ~ ψ := semDtxt.trans hφψ.sym hφψ
+    apply ℰ.trans (ihn (zero_le δ) nj (wtK.letin ahm) rfl hστ hφψ)
+    apply ℰ.trans (semCom.join aihm (soundCom ahn) hττ hψ₂)
+    apply ℰ.trans (joinJoin hm' ahm' ahn hττ hψ₂); simp
     rw [← rejoin.eq_2 _ (m'⦃⇑ τ⦄), ← rejoin.eq_2 _ (m'⦃⇑ τ⦄)]
-    rw [Acom.renameJ (zero_le (δ + 1)) nj rfl]; simp
+    rw [CCcom.renameJ (zero_le (δ + 1)) nj rfl]; simp
     apply ℰ.sym (ihn (zero_le (δ + 1)) nj (.letin ahm') rfl hττ
-      (semDtxt.cons (m := m'⦃⇑ τ⦄) (n := m'⦃⇑ τ⦄) (B := B₂) hjs₂₂ (λ hvw ↦ ?_)))
+      (semDtxt.cons (m := m'⦃⇑ τ⦄) (n := m'⦃⇑ τ⦄) (B := B₂) hψ₂ (λ hvw ↦ ?_)))
     rw [substUnion, substUnion]
-    exact soundCom hm' (semCtxt.cons hvw hττ) hjs₂₂
+    exact soundCom hm' (semCtxt.cons hvw hττ) hψ₂
   case case hv hm₁ hm₂ ih₁ ih₂ =>
-    intro hστ js₁ js₂ hjs; simp; rw [e]
+    intro hστ φ ψ hφψ; simp; rw [e]
     let ⟨vj, mj₁, mj₂⟩ := mj
     split; contradiction
     case _ eyes =>
@@ -187,13 +187,13 @@ theorem semJumpA {Γ δ δ'} {Δ : Dtxt δ} {Δ' : Dtxt δ'} {k k' m m' B₁ B�
         rw [e₁, e₂]
         refine ℰ.bwd (.rejoin .ιl) (.rejoin (.join .ιl)) ?_
         rw [substUnion, substUnion]
-        have hB₂ := h₁ v w (semCtxt.cons hA hστ) hjs
+        have hB₂ := h₁ v w (semCtxt.cons hA hστ) hφψ
         simp at hB₂; rw [renameUpSubstConsVal] at hB₂; exact hB₂
       | .inr ⟨v, w, hA, e₁, e₂⟩ =>
         rw [e₁, e₂]
         refine ℰ.bwd (.rejoin .ιr) (.rejoin (.join .ιr)) ?_
         rw [substUnion, substUnion]
-        have hB₂ := h₂ v w (semCtxt.cons hA hστ) hjs
+        have hB₂ := h₂ v w (semCtxt.cons hA hστ) hφψ
         simp at hB₂; rw [renameUpSubstConsVal] at hB₂; exact hB₂
     case _ eyes =>
       cases eyes; split
@@ -205,7 +205,7 @@ theorem semJumpA {Γ δ δ'} {Δ : Dtxt δ} {Δ' : Dtxt δ'} {k k' m m' B₁ B�
         exact soundCom
           (.join hm' (.case (ValWt.preservation vj hv)
             (ComWt.preservation (.step le) mj₁ (wtK.weaken hk') hm₁)
-            (ComWt.preservation (.step le) mj₂ (wtK.weaken hk') hm₂))) hστ hjs
+            (ComWt.preservation (.step le) mj₂ (wtK.weaken hk') hm₂))) hστ hφψ
       case _ jumpn't eyes =>
         let ⟨_, e⟩ := Jump.repeat e
         rw [e] at eyes; cases eyes; cases jumpn't _ _ rfl
@@ -223,14 +223,14 @@ theorem soundA {Γ} :
   mutual_induction h, h
   all_goals intro σ τ; try subst eq
   case force ih _ =>
-    refine hk.plug (λ hστ js₁ js₂ _ ↦ ?_)
-    cases js₁; cases js₂
+    refine hk.plug (λ hστ φ ψ _ ↦ ?_)
+    cases φ; cases ψ
     unfold semVal 𝒱 at ih
     let ⟨m, n, h, em, en⟩ := ih mj hστ; simp [em, en]
     refine ℰ.bwd .π .π ?_; simp [weakenJCom0, h]
   case lam ih _ =>
-    refine hk.plug (λ hστ js₁ js₂ _ ↦ ?_)
-    cases js₁; cases js₂
+    refine hk.plug (λ hστ φ ψ _ ↦ ?_)
+    cases φ; cases ψ
     refine ℰ.lam (λ v w hA ↦ ?_)
     rw [substUnion, substUnion]
     have goal := ih rfl mj .nil .nil (soundK .nil) (semCtxt.cons hA hστ) .nil
@@ -239,8 +239,8 @@ theorem soundA {Γ} :
     let ⟨mj, vj⟩ := mj
     exact ihm rfl mj (.app hv wtk₁) (.app (.preservation vj hv) wtk₂) (semK.app (ihv vj) hk)
   case ret ih _ =>
-    refine hk.plug (λ hστ js₁ js₂ _ ↦  ?_)
-    cases js₁; cases js₂
+    refine hk.plug (λ hστ φ ψ _ ↦  ?_)
+    cases φ; cases ψ
     exact ℰ.ret (ih mj hστ)
   case letin hn ihn Δ' _ hm ihm =>
     cases Δ'; let ⟨nj, mj⟩ := mj
@@ -251,11 +251,11 @@ theorem soundA {Γ} :
       (semK.letin (ihm rfl mj wtk₁.weaken wtk₂.weaken hk.weaken))
   case case Γ v A₁ A₂ B₁ hv ihv Δ' m n hm₁ hm₂ ihm₁ ihm₂ =>
     cases Δ'; let ⟨vj, mj₁, mj₂⟩ := mj
-    refine semCom.trans (semKcase wtk₁ (.case hv hm₁ hm₂)) (λ hστ js₁ js₂ hjs ↦ ?_)
+    refine semCom.trans (semKcase wtk₁ (.case hv hm₁ hm₂)) (λ hστ φ ψ hφψ ↦ ?_)
     unfold semVal 𝒱 at ihv
     match ihv vj hστ with
     | .inl ⟨v, w, hA₁, ev, ew⟩ =>
-      have hB₂ := ihm₁ rfl mj₁ wtk₁.weaken wtk₂.weaken hk.weaken (semCtxt.cons hA₁ hστ) hjs
+      have hB₂ := ihm₁ rfl mj₁ wtk₁.weaken wtk₂.weaken hk.weaken (semCtxt.cons hA₁ hστ) hφψ
       simp; split <;> simp [ev, ew]
       case _ | _ =>
         refine ℰ.bwd (.rejoin .ιl) (.rejoin .ιl) ?_
@@ -267,12 +267,12 @@ theorem soundA {Γ} :
         rw [substUnion, substUnion]
         refine ℰ.trans hB₂ ?_
         have goal :=
-          semJumpA (zero_le δ) mj₁ wtk₂.weaken hm₁ (Jump.rename e)
+          semJumpCC (zero_le δ) mj₁ wtk₂.weaken hm₁ (Jump.rename e)
             (semCtxt.trans (semCtxt.sym (semCtxt.cons hA₁ hστ)) (semCtxt.cons hA₁ hστ))
-            (semDtxt.trans (semDtxt.sym hjs) hjs)
+            (semDtxt.trans (semDtxt.sym hφψ) hφψ)
         simp [renameUpSubstConsCom] at goal; exact goal
     | .inr ⟨v, w, hA₂, ev, ew⟩ =>
-      have hB₂ := ihm₂ rfl mj₂ wtk₁.weaken wtk₂.weaken hk.weaken (semCtxt.cons hA₂ hστ) hjs
+      have hB₂ := ihm₂ rfl mj₂ wtk₁.weaken wtk₂.weaken hk.weaken (semCtxt.cons hA₂ hστ) hφψ
       simp; split <;> simp [ev, ew]
       case _ | _ =>
         refine ℰ.bwd (.rejoin .ιr) (.rejoin .ιr) ?_
@@ -284,14 +284,14 @@ theorem soundA {Γ} :
         rw [substUnion, substUnion]
         refine ℰ.trans hB₂ ?_
         have goal :=
-          semJumpA (zero_le δ) mj₂ wtk₂.weaken hm₂ (Jump.rename e)
+          semJumpCC (zero_le δ) mj₂ wtk₂.weaken hm₂ (Jump.rename e)
             (semCtxt.trans (semCtxt.sym (semCtxt.cons hA₂ hστ)) (semCtxt.cons hA₂ hστ))
-            (semDtxt.trans (semDtxt.sym hjs) hjs)
+            (semDtxt.trans (semDtxt.sym hφψ) hφψ)
         simp [renameUpSubstConsCom] at goal; exact goal
   case prod ihn₁ ihn₂ _ =>
     let ⟨nj₁, nj₂⟩ := mj
-    refine hk.plug (λ hστ js₁ js₂ _ ↦ ?_)
-    cases js₁; cases js₂; simp
+    refine hk.plug (λ hστ φ ψ _ ↦ ?_)
+    cases φ; cases ψ; simp
     have hB₁ := ihn₁ rfl nj₁ .nil .nil (soundK .nil) hστ .nil
     have hB₂ := ihn₂ rfl nj₂ .nil .nil (soundK .nil) hστ .nil
     simp [weakenJCom0] at hB₁; simp [weakenJCom0] at hB₂
@@ -309,8 +309,8 @@ theorem soundA {Γ} :
     simp [weakenJCom0] at goal; exact 𝒱.thunk goal
 
 theorem soundAnil {Γ m B} (mj : m.joinless) (h : Γ ∣ ⬝ ⊢ m ∶ B) : Γ ∣ ⬝ ⊨ m ~ ⟦m⟧ₘ ∶ B := by
-  intro σ τ hστ js₁ js₂ hjs
-  have goal := soundA.right rfl mj h .nil .nil semK.nil hστ hjs
+  intro σ τ hστ φ ψ hφψ
+  have goal := soundA.right rfl mj h .nil .nil semK.nil hστ hφψ
   simp at goal; rw [weakenJCom0] at goal; exact goal
 
 /-*-------------------------------------------------------------
